concurrency/dry_context.v
@@ -14,41 +14,41 @@ Module SEM <: Semantics.
                Definition Sem := Asm_EvSem.               
 End SEM.
 
-
-Module DryMachine:= DryMachineShell SEM.
-Module ErasedMachine := ErasedMachineShell SEM.
-Module mySchedule := mySchedule.
-(** DryConc machine instantiated for X86*)
-Module DryConc :=
-  CoarseMachine mySchedule DryMachine.
-
-(** FineConc machine instantiated for X86*)
-Module FineConc :=
-  FineMachine mySchedule DryMachine.
-
-(** X86-SC machine*)
-Module X86SC :=
-  FineMachine mySchedule ErasedMachine.
-
-Parameter initU: mySchedule.schedule.
-Parameter the_program: Asm.program.
-
-Definition init_mem := Genv.init_mem the_program.
-Definition init_perm : option access_map :=
-  match init_mem with
-  | Some m => Some (getCurPerm m)
-  | None => None
-  end.
-
-Definition the_ge := Globalenvs.Genv.globalenv the_program.
-
-Definition coarse_semantics:=
-  DryConc.MachineSemantics initU init_perm.
-
-Definition fine_semantics:=
-  FineConc.MachineSemantics initU init_perm.
-
-Definition x86_sc_semantics :=
-  X86SC.MachineSemantics initU None.
+Module DryContext (SEM : Semantics).
+  Module DryMachine:= DryMachineShell SEM.
+  Module ErasedMachine := ErasedMachineShell SEM.
+  Module mySchedule := mySchedule.
+  (** DryConc machine instantiated for X86*)
+  Module DryConc :=
+    CoarseMachine mySchedule DryMachine.
+  
+  (** FineConc machine instantiated for X86*)
+  Module FineConc :=
+    FineMachine mySchedule DryMachine.
+  
+  (** X86-SC machine*)
+  Module X86SC :=
+    FineMachine mySchedule ErasedMachine.
+  
+  Parameter initU: mySchedule.schedule.
+  Parameter the_program: Asm.program.
+  
+  Definition init_mem := Genv.init_mem the_program.
+  Definition init_perm : option access_map :=
+    match init_mem with
+    | Some m => Some (getCurPerm m)
+    | None => None
+    end.
+  
+  Definition the_ge := Globalenvs.Genv.globalenv the_program.
+  
+  Definition coarse_semantics:=
+    DryConc.MachineSemantics initU init_perm.
+  
+  Definition fine_semantics:=
+    FineConc.MachineSemantics initU init_perm.
+  
+  Definition x86_sc_semantics :=
+    X86SC.MachineSemantics initU None.
   
 
